examples/CADP_Glued.v
@@ -2,147 +2,108 @@ Require Import MEBI.Examples.CADP.
 
 Import Protocol.
 
-Definition do_acquire_inner (c:tm) (s:state) (r:resource)
-  : composition
-  :=
-  let e : env := (s, r) in
-  (* REC_DEF 2 *)
-  let t : tm := unfold (AcquireInnerDef, AcquireInnerBody) AcquireInnerBody in
-  (* ACT READ_LOCKED *)
-  match read_locked e with
-  | None => (PRC (ERR,
-                (add_error (Build_error 40
-                  "do_acquire_inner, read_locked e failed" (Build_error_info None (None, None))) s)),
-                r)
-  | Some e =>
-    (* IF (VAR LOCKED) *)
-    match (get_local_var_value LOCKED (get_state e)) with
-    | BOOL true => (* REC_CALL 2 *) (PRC ((SEQ t c), (get_state e)), get_resource e)
-    | BOOL false => (PRC (c, (get_state e)), get_resource e)
-    | _ => (PRC (ERR,
-                (add_error (Build_error 41
-                  "do_acquire_inner, var locked not bool" (Build_error_info None (None, None))) (get_state e))),
-                get_resource e)
-    end
+Definition return_error' (n:nat) (m:string) (s:state) (r:resource) : composition := (PRC (ERR, (add_error (Build_error n m (Build_error_info None (None, None))) s)), r).
+
+
+Definition do_acquire_inner (c:tm) (s:state) (r:resource) : composition :=
+(* REC_DEF 2 *)
+(* let t : tm := unfold (AcquireInnerDef, AcquireInnerBody) AcquireInnerBody in *)
+let t : tm := AcquireInnerLoop in
+(* ACT READ_LOCKED *)
+match read_locked (s, r) with
+| None => return_error' 40 "do_acquire_inner, read_locked e failed" s r
+| Some (s, r) =>
+  (* IF (VAR LOCKED) *)
+  match value_to_bool_opt (get_local_var_value LOCKED s) with
+  | None => return_error' 41 "do_acquire_inner, var locked not bool" s r
+  | Some true => (* REC_CALL 2 *) (PRC (SEQ t c, s), r)
+  | Some false => (PRC (c, s), r)
   end
-  .
+end.
+
+(* Compute (unfold (AcquireInnerDef, AcquireInnerBody) AcquireInnerBody). *)
 
 
-Definition do_acquire (c:tm) (s:state) (r:resource)
-  : composition
-  :=
-  let e : env := (s, r) in
-  (* ACT (WRITE_NEXT THE_PID NIL) *)
-  match write_next THE_PID NIL e with
-  | None => (PRC (ERR,
-                (add_error (Build_error 50
-                  "do_acquire, write_next THE_PID NIL failed" (Build_error_info None (None, None))) s)),
-                r)
-  | Some e =>
-    (* ACT FETCH_AND_STORE *)
-    let e:env := fetch_and_store e in
-    (* IF (EQ (VAR PREDECESSOR) (VAL NIL)) *)
-    match (get_local_var_value PREDECESSOR (get_state e)) with
-    | NIL => (* OK *) (PRC (c, (get_state e)), get_resource e)
-    | _ =>
-      (* ACT (WRITE_LOCKED THE_PID (BOOL true)) *)
-      match write_locked THE_PID (BOOL true) e with
-      | None => (PRC (ERR,
-                    (add_error (Build_error 52
-                      "do_acquire, write_locked THE_PID (BOOL true) failed" (Build_error_info None (None, None))) (get_state e))),
-                (get_resource e))
-      | Some e =>
-        (* ACT (WRITE_NEXT PREDECESSOR (GET THE_PID)) *)
-        match write_next PREDECESSOR (GET THE_PID) e with
-        | None => (PRC (ERR,
-                      (add_error (Build_error 53
-                        "do_acquire, write_next PREDECESSOR (GET THE_PID) failed" (Build_error_info None (None, None))) (get_state e))),
-                  (get_resource e))
-        | Some e =>
-          (PRC (SEQ (AcquireInnerLoop) c, get_state e)
-          , get_resource e
-          )
-        end
+Definition do_acquire (c:tm) (s:state) (r:resource) : composition :=
+(* ACT (WRITE_NEXT THE_PID NIL) *)
+match write_next THE_PID NIL (s, r) with
+| None => return_error' 42 "do_acquire, write_next THE_PID NIL failed" s r
+| Some (s, r) =>
+  (* ACT FETCH_AND_STORE *)
+  let e_:env := fetch_and_store (s, r) in
+  let s:state := fst e_ in
+  let r:resource := snd e_ in
+  (* IF (EQ (VAR PREDECESSOR) (VAL NIL)) *)
+  match value_to_index_opt (get_local_var_value PREDECESSOR s) with
+  | None => return_error' 43 "do_acquire, PREDECESSOR not INDEX" s r
+  | Some None => (* OK *) (PRC (c, s), r)
+  | Some (Some _i) =>
+    (* ACT (WRITE_LOCKED THE_PID (BOOL true)) *)
+    match write_locked THE_PID (BOOL true) (s, r) with
+    | None => return_error' 44 "do_acquire, write_locked THE_PID (BOOL true) failed" s r
+    | Some (s, r) =>
+      (* ACT (WRITE_NEXT PREDECESSOR (GET THE_PID)) *)
+      match write_next PREDECESSOR (GET THE_PID) (s, r) with
+      | None =>  return_error' 45 "do_acquire, write_next PREDECESSOR (GET THE_PID) failed" s r 
+      | Some (s, r) => (PRC (SEQ (AcquireInnerLoop) c, s), r)
       end
     end
   end
-  .
+end.
 
-Definition do_release_inner (c:tm) (s:state) (r:resource)
-  : composition
-  :=
-  let e : env := (s, r) in
-  (* REC_DEF 1 *)
-  let t : tm := unfold (ReleaseInnerDef, ReleaseInnerBody) ReleaseInnerBody in
-  (* ACT READ_NEXT *)
-  match read_next e with
-  | None => (PRC (ERR,
-                (add_error (Build_error 45
-                  "do_release_inner, read_next e failed" (Build_error_info None (None, None))) s)),
-                r)
-  | Some e =>
-    (* IF (EQ (VAL NIL) (VAR NEXT)) *)
-    match (get_local_var_value NEXT (get_state e)) with
-    | NIL => (* REC_CALL 1 *) (PRC ((SEQ t c), (get_state e)), get_resource e)
-    | _ =>
-      (* ACT (WRITE_LOCKED NEXT (BOOL false)) *)
-      match write_locked NEXT (BOOL false) e with
-      | None => (PRC (ERR,
-                    (add_error (Build_error 46
-                      "do_release_inner, write_locked NEXT (BOOL false) failed" (Build_error_info None (None, None))) (get_state e))),
-                    (get_resource e))
-      | Some e =>
-        (PRC (c, (get_state e)), get_resource e)
-      end
+Definition do_release_inner (c:tm) (s:state) (r:resource) : composition :=
+(* REC_DEF 1 *)
+(* let t : tm := unfold (ReleaseInnerDef, ReleaseInnerBody) ReleaseInnerBody in *)
+let t : tm := ReleaseInnerLoop in
+(* ACT READ_NEXT *)
+match read_next (s, r) with
+| None => return_error' 50 "do_release_inner, read_next e failed" s r
+| Some (s, r) =>
+  (* IF (EQ (VAL NIL) (VAR NEXT)) *)
+  match value_to_index_opt (get_local_var_value NEXT s) with
+  | None => return_error' 51 "do_release_inner, NEXT not INDEX" s r
+  | Some None => (* REC_CALL 1 *) (PRC ((SEQ t c), s), r)
+  | Some (Some _i) =>
+    (* ACT (WRITE_LOCKED NEXT (BOOL false)) *)
+    match write_locked NEXT (BOOL false) (s, r) with
+    | None => return_error' 52 "do_release_inner, write_locked NEXT (BOOL false) failed" s r
+    | Some (s, r) => (PRC (c, s), r)
     end
   end
-  .
+end.
 
-Definition do_release (c:tm) (s:state) (r:resource)
-  : composition
-  :=
-  let e : env := (s, r) in
-  (* ACT READ_NEXT *)
-  match read_next e with
-  | None => (PRC (ERR,
-                (add_error (Build_error 60
-                  "do_release, read_next e failed" (Build_error_info None (None, None))) s)),
-                r)
-  | Some e =>
-    (* IF (EQ (VAL NIL) (VAR NEXT)) *)
-    match (get_local_var_value NEXT (get_state e)) with
-    | NIL =>
-      (* ACT COMPARE_AND_SWAP *)
-      let e:env := compare_and_swap e in
-      (* IF (EQ FLS (VAR SWAP)) *)
-      match (get_local_var_value SWAP (get_state e)) with
-      | BOOL false =>
-        (PRC ((SEQ (ReleaseInnerLoop) c), (get_state e))
-        , get_resource e)
-      | _ => (* OK *) (PRC (c, (get_state e)), get_resource e)
-      end
-
-    | _ =>
-      (* ACT (WRITE_LOCKED NEXT (BOOL false)) *)
-      match write_locked NEXT (BOOL false) e with
-      | None => (PRC (ERR,
-                    (add_error (Build_error 61
-                      "do_release, write_locked NEXT (BOOL false) failed" (Build_error_info None (None, None))) (get_state e))),
-                    (get_resource e))
-      | Some e =>
-        (PRC (c, (get_state e)), get_resource e)
-      end
+Definition do_release (c:tm) (s:state) (r:resource) : composition :=
+(* ACT READ_NEXT *)
+match read_next (s, r) with
+| None => return_error' 53 "do_release, read_next e failed" s r
+| Some (s, r) =>
+  (* IF (EQ (VAL NIL) (VAR NEXT)) *)
+  match value_to_index_opt (get_local_var_value NEXT s) with
+  | None => return_error' 54 "do_release, NEXT not INDEX" s r
+  | Some None => 
+    (* ACT COMPARE_AND_SWAP *)
+    let e_:env := compare_and_swap (s, r) in
+    let s:state := fst e_ in
+    let r:resource := snd e_ in
+    (* IF (EQ FLS (VAR SWAP)) *)
+    match value_to_bool_opt (get_local_var_value SWAP s) with
+    | None => return_error' 55 "do_release, SWAP not BOOL" s r
+    | Some false => (PRC (SEQ (ReleaseInnerLoop) c, s), r)
+    | Some true => (* OK *) (PRC (c, s), r)
+    end
+  | Some (Some _i) =>
+    (* ACT (WRITE_LOCKED NEXT (BOOL false)) *)
+    match write_locked NEXT (BOOL false) (s, r) with
+    | None => return_error' 56 "do_release, write_locked NEXT (BOOL false) failed" s r
+    | Some (s, r) => (PRC (c, s), r)
     end
   end
-  .
+end.
 
 
-Definition do_main_loop (b:tm) (s:state) (r:resource)
-  : composition
-  :=
+Definition do_main_loop (b:tm) (s:state) (r:resource) : composition :=
   (* REC_DEF 0 *)
-  (PRC ((unfold (PMainLoopDef, b) b), s), r)
-  .
+  (PRC ((unfold (PMainLoopDef, b) b), s), r).
 
 Inductive bigstep : composition -> option label -> composition -> Prop :=
 | DO_MAIN_LOOP : forall b s r,
@@ -154,7 +115,7 @@ Inductive bigstep : composition -> option label -> composition -> Prop :=
 | DO_ACQUIRE_INNER : forall c s r,
   bigstep (PRC (SEQ AcquireInnerLoop c, s), r) None (do_acquire_inner c s r)
 | DO_RELEASE_INNER : forall c s r,
-  bigstep (PRC (SEQ (ReleaseInnerLoop) c, s), r) None (do_release_inner c s r)
+  bigstep (PRC (SEQ ReleaseInnerLoop c, s), r) None (do_release_inner c s r)
 | DO_SEQ_ACT_ENTER : forall y s r,
   bigstep (PRC (SEQ (ACT ENTER) y, s), r) (Some (ENTER, (get_pid s))) (PRC (y, s), r)
 | DO_SEQ_ACT_LEAVE : forall y s r,
