examples/Bisimilarity/CADP/Size2/Glued/MutualExclusion/PluginProofs.v
@@ -12,7 +12,7 @@ MeBi Config Output "DecodeResults" False.
 MeBi Config Output "DumpResults" False.
 
 
-MeBi Config Output "Debug" True.
+(* MeBi Config Output "Debug" True. *)
 MeBi Config Output "Info" True.
 MeBi Config Output "DecodeResults" True.
 MeBi Config Output "DumpResults" True.
@@ -37,19 +37,15 @@ MeBi Config Bounds As Num States 2000.
 
 Require Import Logic.
 
-(* MeBi Divider "Examples.Bisimilarity.CADP.Size2.Glued.MutualExclusion". *)
-(* MeBi Run FSM (make_spec 2) Using spec_lts. *)
-(* MeBi Run FSM (compose (create 2 Protocol.P)) Using lts step. *)
-
 
 MeBi Divider "Examples.Bisimilarity.CADP.Size2.Glued.MutualExclusion.bigstep".
-Example wsim_bigstep_spec_lts : weak_sim bigstep spec_lts (compose (create 2 Protocol.P)) (make_spec 2). 
-Proof. MeBi Sim Begin bigstep (compose (create 2 Protocol.P)) And spec_lts (make_spec 2) Using lts step.
+Example wsim_bigstep_spec_lts : weak_sim bigstep spec_lts c2 (make_spec 1). 
+Proof. MeBi Sim Begin bigstep c2 And spec_lts (make_spec 1) Using lts step.
   (* Iteration History: _ <- _ <- _ <- _ *) 
   MeBi Sim Solve 1000. Qed.
 
 MeBi Divider "Examples.Bisimilarity.CADP.Size2.Glued.MutualExclusion.spec_lts".
-Example wsim_spec_lts_bigstep : weak_sim spec_lts bigstep (make_spec 2) (compose (create 2 Protocol.P)). 
-Proof. MeBi Sim Begin spec_lts (make_spec 2) And bigstep (compose (create 2 Protocol.P)) Using lts step.
+Example wsim_spec_lts_bigstep : weak_sim spec_lts bigstep (make_spec 1) c2. 
+Proof. MeBi Sim Begin spec_lts (make_spec 1) And bigstep c2 Using lts step.
   (* Iteration History: _ <- _ <- _ <- _ *) 
   MeBi Sim Solve 1000. Qed.
